steel/Zeta.Steel.MultiSetHash.fsti
@@ -42,14 +42,14 @@ val ms_hashfn (ms: mset)
   : hash_value_t
 
 val lemma_hashfn_empty (_:unit)
-  : Lemma (ensures (ms_hashfn empty = initial_hash))
+  : Lemma (ensures (ms_hashfn empty == initial_hash))
 
 (* adding a new element to a multiset is equivalent to hash_accumulation in the hash domain *)
 val lemma_update  (ms: mset) (ie: i_dom) (se: s_dom {related_msdom se ie})
   : Lemma (ensures (let h = ms_hashfn ms in
                     let ms' = MS.add_elem ms ie in
                     let h' = ms_hashfn ms' in
-                    h' = TSM.update_hash_value h se.r se.t se.tid))
+                    h' == TSM.update_hash_value h se.r se.t se.tid))
 
 (* multiset hash of the union of two multisets is the aggregate hash of their hashes *)
 val lemma_union (ms1 ms2: mset)
@@ -57,9 +57,9 @@ val lemma_union (ms1 ms2: mset)
                     let h1 = ms_hashfn ms1 in
                     let h2 = ms_hashfn ms2 in
                     let h = ms_hashfn ms in
-                    h = aggregate_hashes h1 h2))
+                    h == aggregate_hashes h1 h2))
 
 noeq type ms_hash_collision =
   | MSCollision: s1: mset ->
-                 s2: mset {ms_hashfn s1 = ms_hashfn s2 /\ ~ (s1 == s2)} ->
+                 s2: mset {ms_hashfn s1 == ms_hashfn s2 /\ ~ (s1 == s2)} ->
                  ms_hash_collision
