steel/crypto/EverCrypt.AEAD.fsti
@@ -1,0 +1,84 @@
+module EverCrypt.AEAD
+open Steel.ST.Util
+module R = Steel.ST.Reference
+module A = Steel.ST.Array
+module U32 = FStar.UInt32
+module S = FStar.SizeT
+module U8 = FStar.UInt8
+
+let error_code = U8.t
+
+inline_for_extraction noextract
+let key_size = 16
+
+inline_for_extraction noextract
+let iv_size = 96
+
+inline_for_extraction noextract
+let tag_size = 16
+
+inline_for_extraction noextract
+let bytes = Seq.seq U8.t
+
+inline_for_extraction noextract
+let ebytes = Ghost.erased bytes
+
+inline_for_extraction noextract
+let lbytes l = s:bytes { Seq.length s = l }
+
+inline_for_extraction noextract
+let max_input_length = pow2 31 - 1
+
+val spec (k_bytes:lbytes key_size)
+         (iv_bytes:lbytes 96)
+         (in_bytes:bytes { Seq.length in_bytes <=  max_input_length })
+  : GTot (lbytes tag_size)
+
+
+(* This is the C interface that we're trying to call from Steel 
+
+  EverCrypt_Error_error_code
+  EverCrypt_AEAD_encrypt_expand_aes128_gcm_no_check(
+    uint8_t *k,
+    uint8_t *iv,
+    uint32_t iv_len,
+    uint8_t *ad,
+    uint32_t ad_len,
+    uint8_t *plain,
+    uint32_t plain_len,
+    uint8_t *cipher,
+    uint8_t *tag
+  );
+*)
+
+val encrypt_expand_aes128_gcm_no_check
+      (#k_p:perm)
+      (#k_bytes:ebytes { Seq.length k_bytes == key_size })
+      (k:A.array U8.t)
+      (#iv_p:perm)
+      (#iv_bytes:ebytes { Seq.length iv_bytes == iv_size })
+      (iv:A.array U8.t)
+      (iv_len:U32.t { U32.v iv_len == iv_size } )
+      (#in_p:perm)
+      (#in_bytes:ebytes)
+      (input:A.array U8.t)  //Any constraint on size of input?
+      (input_len:U32.t { A.length input == U32.v input_len /\
+                         U32.v input_len <= max_input_length /\ 
+                         Seq.length in_bytes == U32.v input_len })
+      (plain_unused:R.ref U8.t { plain_unused == R.null }) (* We're not using plain *)
+      (plain_len:U32.t { plain_len = 0ul })
+      (cipher_unused:R.ref U8.t { cipher_unused == R.null }) (* We're not using cipher *)
+      (tag:A.array U8.t { A.length tag == 16 })
+  : STT error_code
+    (requires
+       A.pts_to k k_p k_bytes `star`
+       A.pts_to iv iv_p iv_bytes `star`
+       A.pts_to input in_p in_bytes `star`
+       exists_ (A.pts_to tag full_perm))
+    (ensures fun res ->
+      A.pts_to k k_p k_bytes `star`
+      A.pts_to iv iv_p iv_bytes `star`
+      A.pts_to input in_p in_bytes `star`
+      exists_ (fun out ->
+        A.pts_to tag full_perm out `star`
+        pure (res == 0uy ==>  out == spec k_bytes iv_bytes in_bytes)))
