steel/crypto/Hacl.Hash.Blake2b_256.fsti
@@ -1,0 +1,71 @@
+module Hacl.Hash.Blake2b_256
+
+// This file is here to prevent depending on the actual HACL*
+// repository.  The signatures do not correspond to the ones found in
+// the original HACL* file. Notably, this is a Steel signature,
+// whereas HACL* is verified in Low*
+
+// We take verification as good nonetheless and reconcile these files
+// at link-time.
+
+// In the future, we hope that the hacl-star repository will provided
+// a minimal set of fstis that allow bringing into scope the
+// signatures (only) of the various API functions of EverCrypt, all
+// specified in terms of abstract specifications.
+
+module U8 = FStar.UInt8
+module U32 = FStar.UInt32
+module A = Steel.ST.Array
+module R = Steel.ST.Reference
+open Steel.ST.Util
+
+inline_for_extraction noextract
+let size_nat = n:nat { n <= pow2 32 - 1 }
+
+let size_t = U32.t
+
+let max_output = 64
+
+let bytes = Seq.seq U8.t
+
+let max_key_size = 64
+
+inline_for_extraction noextract
+let lbytes l = s:bytes { Seq.length s = l }
+
+noextract
+val spec :
+    d:bytes
+  -> kk:size_nat{kk <= 64 /\ (if kk = 0 then Seq.length d < pow2 128 else Seq.length d + 128 < pow2 64)}
+  -> k:lbytes kk
+  -> nn:size_nat{1 <= nn /\ nn <= 64} ->
+  GTot (lbytes nn)
+  
+val blake2b 
+    (#sout:Ghost.erased (Seq.seq U8.t))
+    (#in_p:perm)
+    (#in_v:Ghost.erased (Seq.seq U8.t))
+    (nn:size_t{1 <= UInt32.v nn /\ UInt32.v nn <= max_output})
+    (output: A.array U8.t)
+    (ll: size_t)
+    (input: A.array U8.t { U32.v ll <= Seq.length in_v })
+    (kk: size_t { U32.v kk <= 64 })
+    (#k_p:perm)
+    (#k_v:Ghost.erased (Seq.seq U8.t) { Seq.length k_v == U32.v kk })
+    (key: A.array U8.t)
+ : ST unit
+    (A.pts_to output full_perm sout `star`
+     A.pts_to input in_p in_v `star`
+     A.pts_to key k_p k_v)
+    (fun _ -> 
+      A.pts_to output full_perm
+               (spec (Seq.slice in_v 0 (U32.v ll))
+                     0
+                     Seq.empty
+                     (UInt32.v nn)) `star`
+      A.pts_to input in_p in_v `star`
+      A.pts_to key k_p k_v)
+  (requires
+    A.length output = U32.v nn)
+  (ensures fun _ ->
+    True)
